extra/ExampleROMore.v
@@ -1,0 +1,391 @@
+
+
+
+
+
+
+
+
+(*-----------LATER using LambdaCFRO
+
+(* ********************************************************************** *)
+(* * Formalisation of records *)
+
+(* ---------------------------------------------------------------------- *)
+(** Read to a record field *)
+
+Definition val_get_field (k:field) :=
+  ValFun 'p :=
+    Let 'q := val_ptr_add 'p (nat_to_Z k) in
+    val_get 'q.
+
+Lemma rule_get_field : forall l k v,
+  triple ((val_get_field k) l)
+    (l `.` k ~~~> v)
+    (fun r => \[r = v] \* (l `.` k ~~~> v)).
+Proof using.
+  intros. applys rule_app_fun. reflexivity. simpl.
+  applys rule_let. { xapplys rule_ptr_add_nat. }
+  intros r. simpl. xpull. intro_subst.
+  rewrite hfield_eq_fun_hsingle.
+  xpull ;=> N. xapplys~ rule_get.
+Qed.
+
+
+(* ---------------------------------------------------------------------- *)
+(** Write to a record field *)
+
+Definition val_set_field (k:field) :=
+  ValFun 'p 'v :=
+    Let 'q := val_ptr_add 'p (nat_to_Z k) in
+    val_set 'q 'v.
+
+Lemma rule_set_field : forall v' l k v,
+  triple ((val_set_field k) l v)
+    (l `.` k ~~~> v')
+    (fun r => (l `.` k ~~~> v)).
+Proof using.
+  intros. applys rule_app_fun2. reflexivity. auto. simpl.
+  applys rule_let. { xapplys rule_ptr_add_nat. }
+  intros r. simpl. xpull. intro_subst.
+  rewrite hfield_eq_fun_hsingle.
+  xpull ;=> N. xapplys~ rule_set.
+Qed.
+
+Arguments rule_set_field : clear implicits.
+
+
+
+(* ********************************************************************** *)
+(* * List cells *)
+
+(* ---------------------------------------------------------------------- *)
+(** Representation *)
+
+(** Identification of head and tail fields *)
+
+Definition hd : field := 0%nat.
+Definition tl : field := 1%nat.
+
+(** [Mcell v q p] describes one list cell allocated at address [p],
+  with head value [v] and tail value [q]. *)
+
+Definition MCell (v:val) (q:val) (p:loc) :=
+  (p `.` hd ~~~> v) \* (p `.` tl ~~~> q).
+
+
+(* ---------------------------------------------------------------------- *)
+(** Tactics *)
+
+(** Tactic hack to make [hsimpl] able to cancel out [hfield]
+    and [Mcell] predicates in heap entailment.
+    Later won't be needed when using [~>] notation. *)
+
+Ltac hcancel_hook H ::=
+  match H with
+  | hsingle _ _ => hcancel_try_same tt
+  | hfield _ _ _ => hcancel_try_same tt
+  | MCell _ _ _ => hcancel_try_same tt
+  end.
+
+
+(* ---------------------------------------------------------------------- *)
+(** Properties of list cells *)
+
+Lemma MCell_eq : forall (v:val) (q:val) (p:loc),
+  MCell v q p = (p `.` hd ~~~> v) \* (p `.` tl ~~~> q).
+Proof using. auto. Qed.
+
+Lemma MCell_inv_not_null : forall p v q,
+  (MCell v q p) ==+> \[p <> null].
+  (* i.e. (MCell v q p) ==> (MCell v q p) \* \[p <> null]. *)
+Proof using.
+  intros. unfold MCell, hd.
+  hchange~ (hfield_not_null p hd). hsimpl~.
+Qed.
+
+Arguments MCell_inv_not_null : clear implicits.
+
+Lemma MCell_null_false : forall v q,
+  (MCell v q null) ==> \[False].
+Proof using. intros. hchanges~ (MCell_inv_not_null null). Qed.
+
+Arguments MCell_null_false : clear implicits.
+
+Lemma MCell_hstar_MCell_inv : forall p1 p2 x1 x2 y1 y2,
+  MCell x1 y1 p1 \* MCell x2 y2 p2 ==+> \[p1 <> p2].
+Proof using.
+  intros. do 2 rewrite MCell_eq. tests C: (p1 = p2).
+  { hchanges (@hstar_hfield_same_loc_disjoint p2 hd). }
+  { hsimpl~. }
+Qed.
+
+
+(* ---------------------------------------------------------------------- *)
+(** Access to list cells *)
+
+(** Read to head *)
+
+Definition val_get_hd := val_get_field hd.
+
+Lemma rule_get_hd : forall p v q,
+  triple (val_get_hd p)
+    (MCell v q p)
+    (fun r => \[r = v] \* (MCell v q p)).
+Proof using.
+  intros. unfold MCell. xapplys rule_get_field. auto.
+Qed.
+
+Hint Extern 1 (Register_spec val_get_hd) => Provide rule_get_hd.
+
+(** Read to tail *)
+
+Definition val_get_tl := val_get_field tl.
+
+Lemma rule_get_tl : forall p v q,
+  triple (val_get_tl p)
+    (MCell v q p)
+    (fun r => \[r = q] \* (MCell v q p)).
+Proof using.
+  intros. unfold MCell.
+  xapplys rule_get_field. auto.
+Qed.
+
+Hint Extern 1 (Register_spec val_get_tl) => Provide rule_get_tl.
+
+(** Write to head *)
+
+Definition val_set_hd := val_set_field hd.
+
+Lemma rule_set_hd : forall p v' v vq,
+  triple (val_set_hd p v)
+    (MCell v' vq p)
+    (fun r => MCell v vq p).
+Proof using.
+  intros. unfold MCell. xapplys (rule_set_field v'). auto.
+Qed.
+
+Hint Extern 1 (Register_spec val_set_hd) => Provide rule_set_hd.
+
+(** Write to tail *)
+
+Definition val_set_tl := val_set_field tl.
+
+Lemma rule_set_tl : forall p v q vq',
+  triple (val_set_tl p q)
+    (MCell v vq' p)
+    (fun r => MCell v q p).
+Proof using.
+  intros. unfold MCell. xapplys (rule_set_field vq'). auto.
+Qed.
+
+Hint Extern 1 (Register_spec val_set_tl) => Provide rule_set_tl.
+
+
+(* ---------------------------------------------------------------------- *)
+(** Allocation of list cells *)
+
+Definition val_new_cell :=
+  ValFun 'x 'y :=
+    Let 'p := val_alloc 2 in
+    val_set_hd 'p 'x;;;
+    val_set_tl 'p 'y;;;
+    'p.
+
+Lemma rule_alloc_cell :
+  triple (val_alloc 2)
+    \[]
+    (fun r => Hexists (p:loc), Hexists v1 v2,
+              \[r = p] \* MCell v1 v2 p).
+Proof using.
+  xapply rule_alloc. { math. } { hsimpl. }
+  { intros r. hpull ;=> l (E&N). subst.
+    simpl_abs. rew_Alloc. hpull ;=> v1 v2.
+    unfold MCell. rewrite hfield_eq_fun_hsingle.
+    unfold hd, tl. hsimpl~ l v1 v2.
+    math_rewrite (l + 1 = S l)%nat.
+    math_rewrite (l+0 = l)%nat. hsimpl. }
+Qed.
+
+Lemma rule_new_cell : forall v q,
+  triple (val_new_cell v q)
+    \[]
+    (fun r => Hexists p, \[r = val_loc p] \* MCell v q p).
+Proof using.
+  intros. xcf. xapp rule_alloc_cell.
+  intros p p' v' q'. intro_subst.
+  xapps~. xapps~. xvals~.
+Qed.
+
+(* TODO: update?
+Lemma rule_new_cell : forall v q,
+  triple (val_new_cell v q)
+    \[]
+    (fun r => Hexists p, \[r = val_loc p] \* MCell v q p).
+Proof using.
+  intros. applys rule_app_fun2. reflexivity. auto. simpl.
+  applys rule_let. { applys rule_alloc_cell. }
+  intros p. xpull ;=> p' v' q'. intro_subst. simpl.
+  applys rule_seq. { xapplys rule_set_hd. }
+  applys rule_seq. { xapplys rule_set_tl. }
+  applys rule_val. hsimpl. auto.
+Qed.
+*)
+
+Hint Extern 1 (Register_spec val_new_cell) => Provide rule_new_cell.
+
+Global Opaque MCell_eq.
+
+
+(* ********************************************************************** *)
+(* * Mutable lists Segments *)
+
+(* ---------------------------------------------------------------------- *)
+(** Representation *)
+
+Fixpoint MListSeg (q:loc) (L:list val) (p:loc) : hprop :=
+  match L with
+  | nil => \[p = q]
+  | x::L' => Hexists (p':loc), (MCell x p' p) \* (MListSeg q L' p')
+  end.
+
+(* ---------------------------------------------------------------------- *)
+(** Hack *)
+
+(** Tactic hack to make [hsimpl] able to cancel out [MList]
+    in heap entailment. *)
+
+Ltac hcancel_hook H ::=
+  match H with
+  | hsingle _ _ => hcancel_try_same tt
+  | hfield _ _ _ => hcancel_try_same tt
+  | MCell _ _ _ => hcancel_try_same tt
+ (* TODO  | MList _ _ => hcancel_try_same tt *)
+  | MListSeg _ _ _ => hcancel_try_same tt
+  end.
+
+
+(* ---------------------------------------------------------------------- *)
+(** Properties *)
+
+Section Properties.
+Implicit Types L : list val.
+
+Lemma MListSeg_nil_eq : forall p q,
+  MListSeg q nil p = \[p = q].
+Proof using. intros. unfolds~ MListSeg. Qed.
+
+Lemma MListSeg_cons_eq : forall p q x L',
+  MListSeg q (x::L') p =
+  Hexists (p':loc), MCell x p' p \* MListSeg q L' p'.
+Proof using. intros. unfold MListSeg at 1. simple~. Qed.
+
+Global Opaque MListSeg.
+
+Lemma MListSeg_nil : forall p,
+  \[] ==> MListSeg p nil p.
+Proof using. intros. rewrite MListSeg_nil_eq. hsimpl~. Qed.
+
+Lemma MListSeg_cons : forall p p' q x L',
+  MCell x p' p \* MListSeg q L' p' ==> MListSeg q (x::L') p.
+Proof using. intros. rewrite MListSeg_cons_eq. hsimpl. Qed.
+
+Lemma MListSeg_one : forall p q x,
+  MCell x q p ==> MListSeg q (x::nil) p.
+Proof using.
+  intros. hchange (@MListSeg_nil q). hchange MListSeg_cons. hsimpl.
+Qed.
+
+Lemma MListSeg_concat : forall p1 p2 p3 L1 L2,
+  MListSeg p2 L1 p1 \* MListSeg p3 L2 p2 ==> MListSeg p3 (L1++L2) p1.
+Proof using.
+  intros. gen p1. induction L1 as [|x L1']; intros.
+  { rewrite MListSeg_nil_eq. hpull ;=> E. subst. rew_list~. }
+  { rew_list. hchange (MListSeg_cons_eq p1). hpull ;=> p1'.
+    hchange (IHL1' p1'). hchanges (@MListSeg_cons p1). }
+Qed.
+
+Lemma MListSeg_last : forall p1 p2 p3 x L,
+  MListSeg p2 L p1 \* MCell x p3 p2 ==> MListSeg p3 (L&x) p1.
+Proof using.
+  intros. hchange (@MListSeg_one p2). hchanges MListSeg_concat.
+Qed.
+
+Lemma MListSeg_then_MCell_inv_neq : forall p q L v1 v2,
+  MListSeg q L p \* MCell v1 v2 q ==>
+  MListSeg q L p \* MCell v1 v2 q \* \[L = nil <-> p = q].
+Proof using.
+  intros. destruct L.
+  { rewrite MListSeg_nil_eq. hsimpl*. split*. (* TODO: why not proved? *) }
+  { rewrite MListSeg_cons_eq. hpull ;=> p'. tests: (p = q).
+    { hchanges (@MCell_hstar_MCell_inv q). }
+    { hsimpl. split; auto_false. } }
+Qed.
+
+End Properties.
+
+Arguments MListSeg_then_MCell_inv_neq : clear implicits.
+
+
+
+
+(* ********************************************************************** *)
+(* * Mutable queue *)
+
+(* ---------------------------------------------------------------------- *)
+(** Representation *)
+
+Definition MQueue (L:list val) (p:loc) :=
+  Hexists (pf:loc), Hexists (pb:loc), Hexists (vx:val), Hexists (vy:val),
+    MCell pf pb p \* MListSeg pb L pf \* MCell vx vy pb.
+
+
+(* ---------------------------------------------------------------------- *)
+(** Copy *)
+
+Parameter val_mqueue_copy : val.
+
+Parameter rule_mqueue_copy : forall p (L:list val),
+  triple (val_mqueue_copy p)
+    PRE (RO (p ~> MList L))
+    POST (fun r => Hexists p', \[r = val_loc p'] \* (p' ~> MList L)).
+
+Hint Extern 1 (Register_spec val_mqueue_copy) => Provide rule_mqueue_copy.
+
+
+(* ---------------------------------------------------------------------- *)
+(** Transfer *)
+
+Parameter val_transfer : val.
+
+Parameter rule_transfer : forall L1 L2 p1 p2,
+  triple (val_transfer p1 p2)
+    PRE (p1 ~> MQueue L1 \* p2 ~> MQueue L2)
+    POST (fun r => p1 ~> MQueue (L1 ++ L2) \* p2 ~> MQueue nil).
+
+Hint Extern 1 (Register_spec val_transfer) => Provide rule_transfer.
+
+
+(* ---------------------------------------------------------------------- *)
+(** Copy-Transfer *)
+
+Definition val_copy_transfer :=
+  ValFun 'p1 'p2 :=
+    Let 'p3 := val_mqueue_copy 'p2 in
+    val_transfer 'p1 'p3.
+
+Lemma rule_copy_transfer : forall L1 L2 p1 p2,
+  triple (val_transfer p1 p2)
+    PRE (p1 ~> MQueue L1 \* RO(p2 ~> MQueue L2))
+    POST (fun r => p1 ~> MQueue (L1 ++ L2)).
+Proof using.
+
+
+Qed.
+
+
+Hint Extern 1 (Register_spec val_copy_transfer) => Provide rule_copy_transfer.
+
+
+*)
+
