export/credits_sep_jar_2017/README.md
@@ -1,0 +1,98 @@
+# --- This file is a snapshot of README.md as of 2018-05-29,
+#     truncated to keep only the relevant information. ---
+
+#############################################################
+# Installation
+
+Installation using opam.
+
+
+```
+   # create an opam switch for CFML2
+   opam switch cfml_8.7.2 -A 4.05.0
+   `opam config env`
+
+   # install Coq at the right version
+   opam pin add coq 8.7.2
+   opam install coqide
+
+   # install TLC from package
+   opam repo add coq-released http://coq.inria.fr/opam/released
+   opam update
+   opam install coq-tlc.20180316  
+
+   # compile CFML2
+   cd ~/cfml2
+   make
+   # alternative: make -j4
+
+```
+
+
+Remarks:
+
+* The general-purpose Coq library called TLC is required for all files.
+  It is available from opam (package name "coq-tlc").
+  
+  Alternatively, one can also use TLC from sources:
+     https://gitlab.inria.fr/charguer/tlc
+  in which case you'll to add a file "settings.sh" with contents, e.g.
+  "TLC=~/tlc/src"
+
+
+
+
+#############################################################
+# Models of Separation Logics for a simple imperative lambda-calculus
+
+This archive contains definitions and proofs of soundness for several
+Separation Logics.
+
+The plain Separation Logic and the characteristic formulae
+(used for more smoothly integrating Separation Logic into interactive
+proofs) is close to that described in Arthur Charguéraud's lecture notes, 
+available from:
+  http://www.chargueraud.org/teach/verif/seplogic.pdf
+
+The Separation Logic equipped with read-only permissions is described in:
+__Temporary Read-Only Permissions for Separation Logic__
+by Arthur Charguéraud and François Pottier
+(ESOP 2017).
+  http://www.chargueraud.org/research/2017/readonlysep/readonlysep.pdf
+
+
+#############################################################
+# Organisation of the directory:
+
+
+## Common files
+
+ * The file __TLCbuffer.v__
+   contains scripts to be later merged into TLC.
+
+ * The file __Fmap.v__
+   defines a representation of finite maps, used to represent stores.
+
+ * The file __SepFunctor.v__
+   contains a functor with derived properties for Separation Logic.
+
+ * The file __LambdaSemantics.v__
+   defines the syntax and semantics of an imperative lambda-calculus.
+
+
+## Plain SL
+
+ * The file __LambdaSep.v__
+   defines a plain Separation Logic (and proves its soundness).
+
+ * The file __LambdaCFTactics.v__
+   defines notation and tactics for characteristic formulae.
+
+## Read-only SL
+
+ * The file __LambdaSepRO.v__
+   defines a Separation Logic with read-only permissions.
+
+ * The file __ExampleRO.v__
+   gives examples of proofs using RO logic.
+
