export/export_common.sh
@@ -1,0 +1,72 @@
+#!/bin/bash
+
+set -euo pipefail
+
+# This script creates a self-contained archive containing a subset
+# of the root directory related to the Iris proof mode.
+
+#############################################################
+
+# The name of the archive to create must be set, e.g.
+# TARGET="credits_sep"
+
+if [ -z "$TARGET" ]; then
+   echo "TARGET not set";
+   exit 1
+fi
+
+#############################################################
+
+
+# The absolute name of the archive directory.
+ARCHIVE=`pwd`/$TARGET
+
+# The absolute name of the local folder.
+LOCAL=`pwd`
+
+# The absolute name of the root folder.
+SOURCES=`pwd`/../..
+
+# Wipe out a previous archive.
+rm -rf $ARCHIVE $ARCHIVE.tar.gz
+
+# Create the archive folder
+mkdir $ARCHIVE
+echo "Copying files into $ARCHIVE"
+
+# Copy Makefile from the root as Makefile.main in the archive
+cp $SOURCES/Makefile $ARCHIVE/Makefile.main
+
+# Copy local Makefile and README.md in the archive
+cp $LOCAL/Makefile $ARCHIVE
+cp $LOCAL/README.md $ARCHIVE
+
+# The list of files to export is read from the local Makefile
+FILES_FROM_MAKEFILE=`sed -n -e '/SRC_FORCE := /p' Makefile`
+FILES=$(echo $FILES_FROM_MAKEFILE| cut -d'=' -f 2)
+
+# Copy a subset of CFML/model into the archive.
+for i in ${FILES} ; do
+  cp $SOURCES/$i.v $ARCHIVE ;
+done
+
+# Add a HASH (current git hash) and DATE file to record the version
+HASH="git log -1 --pretty=%H"
+DATE="/bin/date +%Y%m%d"
+(cd $SOURCES && $HASH) > $ARCHIVE/HASH
+$DATE > $ARCHIVE/DATE
+
+# Create a .tar.gz file
+echo "Creating $TARGET.tar.gz with contents:"
+tar -cvzf $TARGET.tar.gz $TARGET
+
+# Try to compile.
+echo "Testing installation..."
+make -C $TARGET -j4
+echo "---Success!---"
+read -n 1 -p "Press ENTER to delete test folder, or Ctrl+C to keep the files."
+rm -Rf $TARGET
+echo "Cleared $TARGET."
+
+
+
