export/read_only_sep_esop_2017/export.sh
@@ -1,7 +1,7 @@
 #!/bin/bash
 
 # The name of the archive to create
-TARGET="cfml2_mosel"
+TARGET="read_only_sep"
 
 source ../export_common.sh
 
